@@ -1,0 +1,10 @@
+/-
+`argfd` meets its specification, given `argint` and `myproc`.
+-/
+import Xv6.ProofArgfd
+
+namespace Xv6
+
+theorem Argfd (AI : ARGINT) (MP : MYPROC) : ARGFD := argfd_proof AI MP
+
+end Xv6
